SkLean/Preservation.lean
@@ -15,30 +15,115 @@ import Mathlib.Tactic
 /-
 ## Preservation of typing judgements
 
-For unevaluable expressions, the judgement is trivially held. I define convenience lemmas for extracing the type ∀ for the left hand side of a function call and the type of the rhs.
+For unevaluable expressions, the judgement is trivially held. The judgement is also trivially held for application of the \\(K\\) combinator.
+
+I set up some convenience lemmas to prove prservation. Type equivalence of a well-typed `K α β x y` call with the type α and its evaluation are established using these lemmas: if `(K α β x y) : α` and `(K α β x y).eval_once : α`, then the typing α is preserved.
 -/
 
-lemma match_judgement_call (ctx : Ctx) : ∀ (call : Call) (t : SkExpr), valid_judgement ctx (.call call) t → ∃ bind_ty t_body_old, valid_judgement ctx call.lhs (.fall (.mk bind_ty t_body_old)) ∧ valid_judgement ctx call.rhs bind_ty := by
-  intro c t h_judgement_t
-  cases h_judgement_t
-  case call t_lhs h_t_lhs h_t_rhs h_t =>
-    match h : t_lhs with
-      | .mk bind_ty ty_body_old =>
-        use bind_ty
-        use ty_body_old
-        simp_all
-        unfold Fall.bind_ty at h_t_rhs
-        simp at h_t_rhs
-        exact h_t_rhs
-  case beta_eq t₂ h_judgement_t₂ h_beta_eq =>
-    
+lemma k_def_eq : ∀ α β x y, (Call.mk SK[(((K α) β) x)] y).eval_once = x := by
+  intro α β x y
+  unfold Call.eval_once
+  repeat unfold NamedSkExpr.to_sk_expr
+  simp
 
-lemma judgement_holds_eval_once (ctx : Ctx) : ∀ (e : Call) (t : SkExpr), valid_judgement ctx (.call call) t ↔ valid_judgement ctx call.eval_once t := by
-  intro c t
-  constructor
+lemma s_def_eq : ∀ α β γ x y z, (Call.mk SK[(((((S α) β) γ) x) y)] z).eval_once = SK[((x z)(y z))] := by
+  intro α β x y γ
+  unfold Call.eval_once
+  repeat unfold NamedSkExpr.to_sk_expr
+  simp
+
+lemma type_k_eval_def_eq (ctx : Ctx) : ∀ α β x y, valid_judgement ctx x α → valid_judgement ctx (Call.mk SK[(((K α) β) x)] y).eval_once α := by
+  intro α β x y h_t_x
+  unfold Call.eval_once
+  repeat unfold NamedSkExpr.to_sk_expr
+  simp
+  exact h_t_x
+
+/-
+
+## Substitution
+
+This lemma becomes tricky once substitution is required. I prove that all substitutions of `(var n) rhs` where `n ≠ 1` are noops. I also prove that all substitutions of `(var 1) rhs) = rhs`.
+-/
+
+lemma substitute_free_noop : ∀ rhs n, n > 1 → Fall.substitute.substitute_e (.var (.mk ⟨n⟩)) ⟨1⟩ rhs = (.var (.mk ⟨n⟩)) := by
+  intro rhs n h_n_gt_1
+  unfold Fall.substitute.substitute_e
+  simp
   intro h
+  simp_all
+
+lemma substitute_bound_1 : ∀ rhs, Fall.substitute.substitute_e (.var (.mk ⟨1⟩)) ⟨1⟩ rhs = rhs.with_indices_plus (.mk 1) := by
+  intro rhs
+  unfold Fall.substitute.substitute_e
+  simp
+
+/-
+
+## K evaluation type preservation
+
+Now, I prove that `valid_judgement SK[K α β x y] α → valid_judgement SK[K α β x y].eval_once α`.
+-/
+
+lemma type_k_def_eq {m n : ℕ} (ctx : Ctx) : ∀ α β x y, valid_judgement ctx α (.ty (.mk m)) → valid_judgement ctx β (.ty (.mk n)) → valid_judgement ctx x α → valid_judgement ctx y β → valid_judgement ctx SK[((((K α) β) x) y)] α := by
+  intro α β x y h_t_α h_t_β h_t_x h_t_y
+  repeat unfold NamedSkExpr.to_sk_expr
+  apply valid_judgement.call ctx (Call.mk SK[(((K α) β) x)] y) α (Fall.mk β α)
+  unfold Call.lhs
+  simp
+  apply valid_judgement.call ctx (Call.mk SK[((K α) β)] x) (SkExpr.fall (Fall.mk β α)) (Fall.mk α SK[∀ y : β, α])
+  repeat unfold NamedSkExpr.to_sk_expr
+  unfold Call.lhs
+  simp
+  apply valid_judgement.call ctx (Call.mk SK[(K α)] β) SK[∀ x : α, ∀ y : β, α] (Fall.mk (.ty (.mk n)) SK[∀ x : α, ∀ y : β, α])
+  unfold Call.lhs
+  simp
+  apply valid_judgement.call ctx (Call.mk (.k .mk) α) SK[∀ β : (Type n), ∀ x : α, ∀ y : β, α] (@ty_k_fall m n)
+  unfold Call.lhs
+  simp
+  rw [← ty_k_def_eq]
+  exact valid_judgement.k ctx (.mk) ty_k m n (rfl)
+  unfold Call.rhs
+  simp
+  unfold ty_k_fall
+  unfold Fall.bind_ty
+  simp
+  exact h_t_α
+  unfold ty_k_fall
+  unfold Fall.body
   
   sorry
+
+lemma type_s_def_eq (ctx : Ctx
+
+lemma k_judgement_holds_eval_once (ctx : Ctx) : ∀ α β x y t, valid_judgement ctx SK[((((K α) β) x) y)] t → valid_judgement ctx (Call.mk SK[(((K α) β) x)] y).eval_once t := by
+  intro α β x y t h_t_holds
+  repeat unfold NamedSkExpr.to_sk_expr at *
+  unfold Call.eval_once
+  simp
+  cases h_t_holds
+  case call t_lhs h_t_lhs h_t_rhs h_t =>
+    unfold Call.lhs at *
+    simp_all
+    unfold Fall.substitute at *
+    cases t_lhs
+    case mk =>
+    simp_all
+    
+    sorry
+  sorry
+
+lemma judgement_holds_eval_once (ctx : Ctx) : ∀ (call : Call) (t : SkExpr), valid_judgement ctx (.call call) t ↔ valid_judgement ctx call.eval_once t := by
+  intro c t
+  unfold Call.eval_once
+  split
+  case h_1 α β x y =>
+    constructor
+    intro h
+    cases h
+    case mp.call =>
+    
+    sorry
 
 lemma eval_once_candidate_iff (ctx : Ctx) : ∀ (call : Call) (t : SkExpr), is_candidate_for_t ctx (.call call) t ↔ is_candidate_for_t ctx (call.eval_once) t := by
   intro e t
